CSE for known builtin functions
This commit extends value numbering with a new kind of equation tracking applications of builtin functions with known semantics.

It then extends the CSE optimization to reuse results of `Ibuiltin(EF_builtin)` for known builtin functions, just like we do for `Iop` and `Iload`.

backend/CSE.v
@@ -15,7 +15,7 @@
 
 Require Import Coqlib Maps Errors Integers Floats Lattice Kildall.
 Require Import AST Linking Builtins.
-Require Import Values Memory.
+Require Import Values Memory Events.
 Require Import Op Registers RTL.
 Require Import ValueDomain ValueAnalysis CSEdomain CombineOp.
 
@@ -65,6 +65,39 @@ Fixpoint valnum_regs (n: numbering) (rl: list reg)
   | r1 :: rs =>
       let (n1, v1) := valnum_reg n r1 in
       let (ns, vs) := valnum_regs n1 rs in
+      (ns, v1 :: vs)
+  end.
+
+Fixpoint valnum_builtin_arg (n: numbering) (a: builtin_arg reg)
+                 {struct a} : numbering * builtin_arg valnum :=
+  match a with
+  | BA r => let (n, v) := valnum_reg n r in (n, BA v)
+  | BA_int i => (n, BA_int i)
+  | BA_long i => (n, BA_long i)
+  | BA_float f => (n, BA_float f)
+  | BA_single f => (n, BA_single f)
+  | BA_loadstack chunk ofs => (n, BA_loadstack chunk ofs)
+  | BA_addrstack ofs => (n, BA_addrstack ofs)
+  | BA_loadglobal chunk id ofs => (n, BA_loadglobal chunk id ofs)
+  | BA_addrglobal id ofs => (n, BA_addrglobal id ofs)
+  | BA_splitlong a1 a2 =>
+      let (n, v1) := valnum_builtin_arg n a1 in
+      let (n, v2) := valnum_builtin_arg n a2 in
+      (n, BA_splitlong v1 v2)
+  | BA_addptr a1 a2 =>
+      let (n, v1) := valnum_builtin_arg n a1 in
+      let (n, v2) := valnum_builtin_arg n a2 in
+      (n, BA_addptr v1 v2)
+  end.
+
+Fixpoint valnum_builtin_args (n: numbering) (args: list (builtin_arg reg))
+               {struct args} : numbering * list (builtin_arg valnum) :=
+  match args with
+  | nil =>
+      (n, nil)
+  | arg1 :: args =>
+      let (n1, v1) := valnum_builtin_arg n arg1 in
+      let (ns, vs) := valnum_builtin_args n1 args in
       (ns, v1 :: vs)
   end.
 
@@ -207,9 +240,20 @@ Definition add_load (n: numbering) (rd: reg)
   let (n1, vs) := valnum_regs n rs in
   add_rhs n1 rd (Load chunk addr vs p).
 
-(** [set_unknown n rd] returns a numbering where [rd] is mapped to
-  no value number, and no equations are added.  This is useful
-  to model instructions with unpredictable results such as [Ibuiltin]. *)
+(** [add_builtin n res bf args] specializes [add_rhs] for the case of a
+  built-in function.  The right-hand side corresponding to [bf]
+  and the value numbers for the argument [args] [rs] is built
+  and added to [n] as described in [add_rhs]. *)
+
+Definition add_builtin (n: numbering) (dst: builtin_res reg)
+                       (bf: builtin_function) (args: list (builtin_arg reg)) :=
+  match dst with
+  | BR rd =>
+      let (n1, args1) := valnum_builtin_args n args in
+      add_rhs n1 rd (Builtin bf args1)
+  | _ =>
+      n
+  end.
 
 Definition set_unknown (n: numbering) (rd: reg) :=
   {| num_next := n.(num_next);
@@ -247,6 +291,7 @@ Definition filter_loads (r: rhs) : bool :=
   match r with
   | Op op _ => op_depends_on_memory op
   | Load _ _ _ _ => true
+  | Builtin bf args => builtin_args_depends_on_memory args
   end.
 
 Definition kill_all_loads (n: numbering) : numbering :=
@@ -264,6 +309,8 @@ Definition filter_after_store (n: numbering) (p: aptr) (sz: Z) (r: rhs) :=
       op_depends_on_memory op
   | Load chunk addr vl q =>
       negb (pdisjoint q (size_chunk chunk) p sz)
+  | Builtin bf args =>
+      builtin_args_depends_on_memory args
   end.
 
 Definition kill_loads_after_store
@@ -435,7 +482,7 @@ Module Solver := BBlock_solver(Numbering).
   Finally, for instructions that modify neither registers nor
   the memory, we keep the numbering unchanged.
 
-  For builtin invocations [Ibuiltin], we have three strategies:
+  For builtin invocations [Ibuiltin], we have four strategies:
 - Forget all equations.  This is appropriate for builtins that can be
   turned into function calls
   ([EF_external], [EF_runtime], [EF_malloc], [EF_free]).
@@ -443,8 +490,9 @@ Module Solver := BBlock_solver(Numbering).
   This is appropriate for builtins that can modify memory,
   e.g. volatile stores, or [EF_builtin] for unknown builtin functions.
 - Keep all equations, taking advantage of the fact that neither memory
-  nor registers are modified.  This is appropriate for annotations,
-  volatile loads, and known builtin functions.
+  nor registers are modified.  This is appropriate for annotations and
+  volatile loads.
+- Keep all equations and add a new equation.  This is for known builtin functions.
 *)
 
 Definition transfer (f: function) (approx: PMap.t VA.t) (pc: node) (before: numbering) :=
@@ -474,7 +522,7 @@ Definition transfer (f: function) (approx: PMap.t VA.t) (pc: node) (before: numb
               set_res_unknown (kill_all_loads before) res
           | EF_builtin name sg =>
               match lookup_builtin_function name sg with
-              | Some bf => set_res_unknown before res
+              | Some bf => add_builtin before res bf args
               | None    => set_res_unknown (kill_all_loads before) res
               end
           | EF_memcpy sz al =>
@@ -511,9 +559,10 @@ Definition analyze (f: RTL.function) (approx: PMap.t VA.t): option (PMap.t numbe
 (** * Code transformation *)
 
 (** The code transformation is performed instruction by instruction.
-  [Iload] instructions and non-trivial [Iop] instructions are turned
-  into move instructions if their result is already available in a
-  register, as indicated by the numbering inferred at that program point.
+  [Iload] instructions, non-trivial [Iop] instructions, and [Ibuiltin]
+  with known built-in functions are turned into move instructions if
+  their result is already available in a register, as indicated by the
+  numbering inferred at that program point.
 
   Some operations are so cheap to compute that it is generally not
   worth reusing their results.  These operations are detected by the
@@ -544,6 +593,17 @@ Definition transf_instr (n: numbering) (instr: instruction) :=
       let (n1, vl) := valnum_regs n args in
       let (addr', args') := reduce _ combine_addr n1 addr args vl in
       Istore chunk addr' args' src s
+  | Ibuiltin (EF_builtin name sg) args (BR res) s =>
+      match lookup_builtin_function name sg with
+      | Some bf =>
+          let (n1, args') := valnum_builtin_args n args in
+          match find_rhs n1 (Builtin bf args') with
+          | Some r => Iop Omove (r :: nil) res s
+          | None   => instr
+          end
+      | None =>
+          instr
+      end
   | Icond cond args s1 s2 =>
       let (n1, vl) := valnum_regs n args in
       match combine_cond' cond vl with
